add acyclic predicate

UnitProJ/expressOS/singleLL/MethodsInINode/INode.dfy
@@ -7,6 +7,19 @@ ghost var footprint: set<INode>;
 var data: Data;
 var next: INode;
 
+predicate acyclic()
+reads *;
+decreases footprint;
+{
+this in footprint 
+&& (next != null ==> (
+	this !in next.footprint 
+  && (( next in footprint &&
+	next.footprint + {this} == footprint && next.acyclic())
+	|| next.Valid())
+	))
+}
+
 predicate good()
 reads this, footprint;
 {
@@ -49,275 +62,48 @@ ensures fresh(footprint - {this});
 	footprint := {this};
 }
 
-}
-
-
-function getFtprint(nd:INode): set<INode>
-reads nd;
+method preAppend(d:Data) returns (node:INode)
+requires Valid();
+ensures node != null && node.Valid();
+ensures node.data == d && node.next == this;
 {
-if nd == null then {} else nd.footprint
+var r := new INode.init(d);
+r.next := this;
+
+r.footprint := r.footprint + this.footprint;
+r.tailContents := [this.data] + this.tailContents;
+return r;
 }
 
-function sumAllFtprint(mySeq: seq<INode>): set<INode>
-reads mySeq;
-ensures forall nd :: nd in mySeq ==> 
-	(nd != null ==> nd.footprint <= sumAllFtprint(mySeq));
+method append(d:Data)
+requires Valid();
+
+modifies footprint;
+decreases footprint;
+ensures Valid();
+ensures (tailContents == old(tailContents) + [d]);
+ensures this.data == old(this.data);
+ensures fresh(footprint - old(footprint));
 {
-if mySeq == [] then {} else getFtprint(mySeq[0]) + sumAllFtprint(mySeq[1..])
-}
+var node := new INode.init(d);
 
-
-/*
-predicate allV(myNode:INode)
-reads myNode, getFtprint(myNode);
-requires myNode != null && myNode.Valid();
-decreases myNode.footprint;
-ensures allV(myNode);
-ensures forall nd :: nd in myNode.footprint ==> nd != null && nd.Valid();
+if(next == null)
 {
-
-if (myNode.next == null)
-then myNode.footprint == {myNode}
-else 
-allV(myNode.next)
+next := node;
+this.tailContents := [d];
 }
 
-
-lemma allValidLemma(myNode:INode)
-requires myNode != null && myNode.Valid();
-requires myNode.next != null ==> myNode.next.Valid();
-decreases myNode.footprint;
-ensures forall nd :: nd in myNode.footprint ==> nd != null && nd.Valid();
-{
-assert allV(myNode);
-}
-*/
-
-predicate seqFtprintLemma(mySeq: seq<INode>)
-requires mySeq != [] && null !in mySeq;
-requires forall nd :: nd in mySeq ==> nd.Valid();
-requires forall i :: 0 <= i < |mySeq|-1 ==> mySeq[i].next == mySeq[i+1];
-requires mySeq[|mySeq|-1].next == null;
-reads mySeq, sumAllFtprint(mySeq);
-ensures seqFtprintLemma(mySeq);
-ensures mySeq[0].footprint == (set nd | nd in mySeq);
-ensures forall nd :: nd in mySeq ==> nd.footprint <= mySeq[0].footprint;
-ensures forall nd :: nd in mySeq[1..] ==> nd.footprint < mySeq[0].footprint;
-{
-if |mySeq| == 1 then true
-else (
-mySeq[0].footprint == {mySeq[0]} + mySeq[1].footprint &&
-seqFtprintLemma(mySeq[1..]))
+else
+ {
+next.append(d);
+this.tailContents := [this.next.data] + this.next.tailContents;
 }
 
-predicate seqV(mySeq: seq<INode>)
-requires goodSeqCond(mySeq);
-requires mySeq != [] ==> mySeq[0].Valid();
+this.footprint := {this} + next.footprint;
 
-reads mySeq, sumAllFtprint(mySeq);
-ensures seqV(mySeq);
-ensures goodSeqCond(mySeq);
-ensures forall nd :: nd in mySeq ==> nd.Valid(); 
-{
-mySeq == [] ||
-(seqV(mySeq[1..]))
 }
 
-
-predicate allNdValid2GoodSeqCond(mySeq: seq<INode>)
-requires seqInv(mySeq);
-requires forall nd :: nd in mySeq ==> nd.Valid();
-requires mySeq != [] ==> mySeq[|mySeq|-1].next == null;
-reads mySeq, sumAllFtprint(mySeq);
-ensures allNdValid2GoodSeqCond(mySeq);
-ensures goodSeqCond(mySeq);
-ensures validSeqCond(mySeq);
-{
-if mySeq == [] then true
-else if |mySeq|==1 then mySeq[0].Valid() && mySeq[0].next == null
-else 
-mySeq[0].next == mySeq[1] && seqFtprintLemma(mySeq) &&
-allNdValid2GoodSeqCond(mySeq[1..])
 }
-
-
-predicate goodSeqCond(mySeq: seq<INode>)
-reads mySeq;
-{
-allDiff(mySeq) &&
-(forall nd :: nd in mySeq ==> nd != null && nd in nd.footprint) &&
-(forall i :: 0 <= i < |mySeq|-1 ==> mySeq[i].next == mySeq[i+1]
-	&& (mySeq != [] ==> mySeq[|mySeq|-1].next !in mySeq)
-	&& mySeq[i].footprint == {mySeq[i]} + mySeq[i+1].footprint) 
-&&(forall i :: 0 <= i < |mySeq| ==> (set nd | nd in mySeq[0..i])					
-				!! mySeq[i].footprint)
-}
-
-predicate validSeqCond(mySeq: seq<INode>)
-reads mySeq;
-{
-goodSeqCond(mySeq) &&
-(forall i, j :: 0 <= i < j < |mySeq| ==> 
-	(mySeq[i].footprint > mySeq[j].footprint)) 
-&& (forall nd :: nd in mySeq ==> 
-    (nd.next == null <==> nd == mySeq[|mySeq|-1])
-    && (nd.next != null <==> exists index :: 0 <= index < |mySeq|-1 
-				&& nd == mySeq[index]))
-}
-
-
-//===============================================
-
-predicate allDiff(mySeq:seq<INode>)
-reads mySeq;
-{
-forall index :: 0 <= index < |mySeq| ==> 
-	(forall other :: 0 <= other < |mySeq| && other != index ==>
-	 (mySeq[other] != mySeq[index]))
-}
-
-
-
-
-
-//==seq invariant inside the loop===
-predicate seqInv(mySeq: seq<INode>)
-reads mySeq;
-{
-allDiff(mySeq) &&
-(forall nd :: nd in mySeq ==> nd != null && nd in nd.footprint) &&
-(forall i :: 0 <= i < |mySeq|-1 ==> mySeq[i].next == mySeq[i+1]) &&
-(mySeq != [] ==> mySeq[|mySeq|-1].next !in mySeq) &&
-(forall i :: 0 <= i < |mySeq| ==> (set nd | nd in mySeq[0..i])					
-				!! mySeq[i].footprint)
-}
-
-/*
-predicate stillSeqInv(mySeq:seq<INode>, newNd:INode)
-requires mySeq != [] && seqInv(mySeq);
-requires newNd != null && newNd.Valid() && newNd.next == mySeq[0];
-requires {newNd} !! sumAllFtprint(mySeq);
-requires forall nd :: nd in mySeq ==> nd.next != newNd;
-reads mySeq, sumAllFtprint(mySeq), newNd, getFtprint(newNd);
-ensures seqInv([newNd]+mySeq);
-{
-true
-}
-*/
-
-/////////////////////////////////////////////////////////////////
-ghost method updateCurIndex(mySeq:seq<INode>, index:int)
-requires 0 <= index <= |mySeq| - 2;
-requires seqInv(mySeq);
-requires mySeq[|mySeq|-1].next == null;
-requires mySeq[index+1].Valid();
-
-requires forall i :: index < i < |mySeq|-1 ==> 
-	(mySeq[i].tailContents == [mySeq[i+1].data] + mySeq[i+1].tailContents)
- && (mySeq[i].footprint == {mySeq[i]} + mySeq[i+1].footprint);
-
-modifies mySeq;
-ensures seqInv(mySeq);
-ensures mySeq[|mySeq|-1].next == null;
-ensures forall i :: index <= i < |mySeq|-1 ==> 
-	(mySeq[i].tailContents == [mySeq[i+1].data] + mySeq[i+1].tailContents)
- && (mySeq[i].footprint == {mySeq[i]} + mySeq[i+1].footprint);
-ensures mySeq[index].Valid();
-{
-mySeq[index].tailContents := [mySeq[index+1].data] + mySeq[index+1].tailContents;
-
-mySeq[index].footprint := {mySeq[index]} + mySeq[index+1].footprint;
-}
-
-//********************************
-//===simulate the loop==
-//*******************************
-ghost method updateSeq(mySeq:seq<INode>)
-
-requires mySeq != [];
-requires seqInv(mySeq);
-requires mySeq[|mySeq|-1].next == null;
-requires mySeq[|mySeq|-1].Valid();
-
-modifies mySeq;
-ensures seqInv(mySeq);
-ensures mySeq[|mySeq|-1].next == null;
-requires mySeq[|mySeq|-1].Valid();
-
-ensures forall i :: 0 <= i < |mySeq|-1 ==> 
-	(mySeq[i].tailContents == [mySeq[i+1].data] + mySeq[i+1].tailContents)
- && (mySeq[i].footprint == {mySeq[i]} + mySeq[i+1].footprint);
-
-ensures forall nd :: nd in mySeq ==> nd.Valid();
-ensures validSeqCond(mySeq);
-
-ensures mySeq[0].footprint == (set nd | nd in mySeq);
-ensures forall nd :: nd in mySeq ==> nd.footprint <= mySeq[0].footprint;
-ensures forall nd :: nd in mySeq[1..] ==> nd.footprint < mySeq[0].footprint;
-{
-ghost var index := |mySeq| - 2;
-
-while(index >= 0)
-invariant -1 <= index <= |mySeq| - 2;
-
-invariant forall i :: index < i < |mySeq|-1 ==> 
-	(mySeq[i].tailContents == [mySeq[i+1].data] + mySeq[i+1].tailContents)
- && (mySeq[i].footprint == {mySeq[i]} + mySeq[i+1].footprint);
-
-invariant seqInv(mySeq);
-invariant mySeq[|mySeq|-1].next == null;
-invariant mySeq[index+1].Valid();
-{
-updateCurIndex(mySeq, index);
-
-index := index - 1;
-
-assert forall i :: index < i < |mySeq|-1 ==> 
-	(mySeq[i].tailContents == [mySeq[i+1].data] + mySeq[i+1].tailContents)
- && (mySeq[i].footprint == {mySeq[i]} + mySeq[i+1].footprint);
-
-assert seqInv(mySeq);  
-assert mySeq[|mySeq|-1].next == null;
-}
-
-assert seqV(mySeq);
-assert allNdValid2GoodSeqCond(mySeq);
-assert seqFtprintLemma(mySeq);
-}
-
-
-lemma setLE(a:set<INode>, b:set<INode>,
-	newA:set<INode>, newB:set<INode>, nd:INode)
-requires a <= b;
-requires newA == a + {nd} && newB == b + {nd};
-ensures newA <= newB;
-{}
-
-
-function ndSeq2DataSeq(mySeq:seq<INode>) : seq<Data>
-requires null !in mySeq;
-reads mySeq;
-ensures |mySeq| == |ndSeq2DataSeq(mySeq)|;
-ensures forall i :: 0 <= i < |mySeq| ==> 
-	ndSeq2DataSeq(mySeq)[i] == mySeq[i].data;
-{
-if mySeq == [] then []
-else [mySeq[0].data] + ndSeq2DataSeq(mySeq[1..])
-}
-
-
-predicate contentOK(oldContent:seq<Data>, oldSpine:seq<INode>,
-			newContent:seq<Data>, newSpine:seq<INode>,
-			newNd:INode, d:Data)
-requires null !in oldSpine && oldSpine != [];
-requires oldContent == ndSeq2DataSeq(oldSpine);
-requires newContent == oldContent + [d];
-requires newNd != null;
-requires newSpine == oldSpine + [newNd] && newNd.data == d;
-reads *;
-ensures newContent == ndSeq2DataSeq(newSpine);
-{true}
-
 
 
 
